Working on the disjoint_memory proof

Compat.v
@@ -4,79 +4,130 @@ From Elo Require Import Array.
 From Elo Require Import Core0.
 From Elo Require Import Access.
 
-Definition compat m m' t := forall ad,
-  access m t ad ->
-  getTM m ad = getTM m' ad.
+Module Compat.
+  Definition compat m m' t := forall ad,
+    access m t ad ->
+    getTM m ad = getTM m' ad.
 
-Lemma compat_symmetry : forall m m' t, 
-  compat m m' t ->
-  compat m' m t. 
-Proof.
-  intros * Hcompat ad Hacc. unfold compat in *.
-  induction Hacc; eauto using access;
-  try solve [symmetry; eauto using access].
-  eapply IHHacc. intros ? ?.
-  eapply Hcompat. eapply access_mem.
-  rewrite (Hcompat _ (access_loc _ _)).
-  trivial.
-Qed.
+  Lemma refl : forall m t, 
+    compat m m t.
+  Proof.
+    intros. unfold compat. trivial.
+  Qed.
 
-Local Lemma compat_access : forall m m' t ad,
-  compat m m' t ->
-  access m t ad ->
-  access m' t ad.
-Proof.
-  intros * Hcompat Hacc. unfold compat in *.
-  induction Hacc; eauto using access.
-  eapply access_mem.
-  rewrite <- (Hcompat _ (access_loc _ _)).
-  eapply IHHacc. intros ? ?.
-  eapply Hcompat. eauto using access.
-Qed.
+  Lemma sym : forall m m' t, 
+    compat m  m' t ->
+    compat m' m  t. 
+  Proof.
+    intros * Hcompat ad Hacc. unfold compat in *.
+    induction Hacc; eauto using access;
+    try solve [symmetry; eauto using access].
+    eapply IHHacc. intros ? ?.
+    eapply Hcompat. eapply access_mem.
+    rewrite (Hcompat _ (access_loc _ _)).
+    trivial.
+  Qed.
 
-Lemma compat_access_symmetry : forall m m' t ad,
-  compat m m' t ->
-  access m t ad <-> access m' t ad.
-Proof.
-  intros * ?. split; eauto using compat_access, compat_symmetry.
-Qed.
+  Lemma acc : forall m m' t ad,
+    compat m m' t ->
+    access m  t ad ->
+    access m' t ad.
+  Proof.
+    intros * Hcompat Hacc. unfold compat in *.
+    induction Hacc; eauto using access.
+    eapply access_mem.
+    rewrite <- (Hcompat _ (access_loc _ _)).
+    eapply IHHacc. intros ? ?.
+    eapply Hcompat. eauto using access.
+  Qed.
 
-Lemma compat_set : forall m m' t ad v,
-  compat m m' t ->
-  ~ access m t ad ->
-  compat m (set m' ad v) t.
-Proof.
-  intros * Hcompat Hnacc ad Hacc. unfold compat in *.
-  induction Hacc. 
-  - eapply IHHacc; eauto using access.
-  - match goal with H : ~ access _ _ ?ad' |- _ => 
-      destruct (Nat.eq_dec ad ad'); subst
-    end.
-    + exfalso. eauto using access.
-    + rewrite (get_set_neq TM_Nil); eauto using access.
-  - eauto using access, inversion_not_access_new.
-  - eauto using access, inversion_not_access_load.
-  - eapply inversion_not_access_asg in Hnacc as [? ?]. eauto using access.
-  - eapply inversion_not_access_asg in Hnacc as [? ?]. eauto using access.
-  - eapply inversion_not_access_seq in Hnacc as [? ?]. eauto using access.
-  - eapply inversion_not_access_seq in Hnacc as [? ?]. eauto using access.
-Qed.
+  Corollary access_symmetry : forall m m' t ad,
+    compat m m' t ->
+    access m t ad <-> access m' t ad.
+  Proof.
+    intros * ?. split; eauto using acc, sym.
+  Qed.
 
-Lemma
+  Lemma inaccessible_address : forall m m' t ad v,
+    compat m m' t ->
+    ~ access m t ad ->
+    compat m (set m' ad v) t.
+  Proof.
+    intros * Hcompat Hnacc ad Hacc. unfold compat in *.
+    induction Hacc; try solve [inversion_not_access; eauto using access].
+    - eapply IHHacc; eauto using access.
+    - match goal with H : ~ access _ _ ?ad' |- _ => 
+        destruct (Nat.eq_dec ad ad'); subst
+      end.
+      + exfalso. eauto using access.
+      + rewrite (get_set_neq TM_Nil); eauto using access.
+  Qed.
+End Compat.
+
+(* changing an inaccessible address does not interfere with access *)
+Lemma access_inaccessible_address : forall m t ad ad' v,
   access m t ad ->
   ~ access m t ad' ->
   access (set m ad' v) t ad.
-Usar o de cima.
-  
+Proof.
+  intros * ? ?.
+  eauto using Compat.refl, Compat.inaccessible_address, Compat.acc.
+Qed.
 
-Def NonInterf m ths := forall tid1 tid2 ad,
-  access m (get tid1) ad ->
-  access m (get tid2) ad ->
+Definition disjoint_memory m ths := forall tid1 tid2 ad,
+  access m (getTM ths tid1) ad ->
+  access m (getTM ths tid2) ad ->
   tid1 = tid2.
 
+Theorem disjoint_memory_preservation : forall m m' ths ths' tid eff,
+  disjoint_memory m ths ->
+  m / ths ~~[tid, eff]~~> m' / ths' ->
+  disjoint_memory m' ths'.
+Proof.
+  intros * Hdis Hcstep tid1 tid2 ad Hacc1 Hacc2.
+  specialize (Hdis tid1 tid2 ad).
+  inversion Hcstep; subst.
+  - clear Hcstep; inversion H1; subst.
+    + destruct (Nat.eq_dec tid tid1) as [? | Hneq]; 
+      destruct (Nat.eq_dec tid tid2);
+      subst; trivial.
+      * exfalso.
+        rewrite (get_set_eq TM_Nil) in Hacc1;
+        rewrite (get_set_neq TM_Nil) in Hacc2;
+        eauto using mstep_none_does_not_grant_access.
+      * exfalso.
+        eapply not_eq_sym in Hneq.
+        rewrite (get_set_eq TM_Nil) in Hacc2;
+        rewrite (get_set_neq TM_Nil) in Hacc1;
+        eauto using mstep_none_does_not_grant_access.
+      * rewrite (get_set_neq TM_Nil) in *; eauto.
+    + admit.
+    + destruct (Nat.eq_dec tid tid1) as [? | Hneq]; 
+      destruct (Nat.eq_dec tid tid2);
+      subst; trivial.
+      * exfalso.
+        rewrite (get_set_eq TM_Nil) in Hacc1;
+        rewrite (get_set_neq TM_Nil) in Hacc2;
+        eauto using mstep_load_does_not_grant_access.
+      * exfalso.
+        eapply not_eq_sym in Hneq.
+        rewrite (get_set_eq TM_Nil) in Hacc2;
+        rewrite (get_set_neq TM_Nil) in Hacc1;
+        eauto using mstep_load_does_not_grant_access.
+      * rewrite (get_set_neq TM_Nil) in *; eauto.
+    + destruct (Nat.eq_dec tid tid1) as [? | Hneq]; 
+      destruct (Nat.eq_dec tid tid2);
+      subst; trivial.
+      * exfalso.
+        rewrite (get_set_eq TM_Nil) in Hacc1;
+        rewrite (get_set_neq TM_Nil) in Hacc2;
+        eauto using mstep_load_does_not_grant_access.
+      * exfalso.
+        eapply not_eq_sym in Hneq.
+        rewrite (get_set_eq TM_Nil) in Hacc2;
+        rewrite (get_set_neq TM_Nil) in Hacc1;
+        eauto using mstep_load_does_not_grant_access.
+      * rewrite (get_set_neq TM_Nil) in *; eauto.
+  - admit.
+Qed.
 
-Lemma  noninterf_preservation
-  has_type t // sí
-  noninter t
-  t --> t'
-  noninter t'
