Access.v
@@ -1,3 +1,7 @@
+From Coq Require Import Arith.Arith.
+
+From Coq Require Logic.ClassicalFacts.
+
 From Elo Require Import Array.
 From Elo Require Import Core0.
 
@@ -43,14 +47,23 @@ Proof.
   intros * Hacc ?. induction Hacc; eauto using access.
 Qed.
 
+Local Axiom excluded_middle : ClassicalFacts.excluded_middle.
+
+Lemma access_dec : forall m t ad,
+  (access m t ad) \/ (~ access m t ad).
+Proof.
+  eauto using excluded_middle.
+Qed.
+
 Ltac inversion_access :=
   match goal with
-    | [ H : access _ TM_Nil _ |- _ ] => inversion H; clear H
-    | [ H : access _ (TM_Num _) _ |- _ ] => inversion H; clear H
-    | [ H : access _ (TM_New _) _ |- _ ] => inversion H; subst; clear H
-    | [ H : access _ (TM_Load _) _ |- _ ] => inversion H; subst; clear H
-    | [ H : access _ (TM_Asg _ _) _ |- _ ] => inversion H; subst; clear H
-    | [ H : access _ (TM_Seq _ _) _ |- _ ] => inversion H; subst; clear H
+    | H : access _ TM_Nil       _ |- _ => inversion H; clear H
+    | H : access _ (TM_Num _)   _ |- _ => inversion H; clear H
+    | H : access _ (TM_Loc _)   _ |- _ => inversion H; clear H
+    | H : access _ (TM_New _)   _ |- _ => inversion H; subst; clear H
+    | H : access _ (TM_Load _)  _ |- _ => inversion H; subst; clear H
+    | H : access _ (TM_Asg _ _) _ |- _ => inversion H; subst; clear H
+    | H : access _ (TM_Seq _ _) _ |- _ => inversion H; subst; clear H
   end.
 
 Lemma inversion_not_access_new : forall m t ad,
@@ -83,44 +96,171 @@ Qed.
 
 Ltac inversion_not_access :=
   match goal with
-    | [ H : ~ access _ (TM_New _) _ |- _ ] =>
-        eapply inversion_not_access_new in H; clear H
-    | [ H : ~ access _ (TM_Load _) _ |- _ ] =>
-        eapply inversion_not_access_load in H; clear H
-    | [ H : ~ access _ (TM_Asg _ _) _ |- _ ] =>
-        eapply inversion_not_access_asg in H; clear H
-    | [ H : ~ access _ (TM_Seq _ _) _ |- _ ] =>
-        eapply inversion_not_access_seq in H; clear H
+    | H : ~ access _ (TM_New _) _   |- _ =>
+        eapply inversion_not_access_new in H
+    | H : ~ access _ (TM_Load _) _  |- _ =>
+        eapply inversion_not_access_load in H
+    | H : ~ access _ (TM_Asg _ _) _ |- _ =>
+        eapply inversion_not_access_asg in H as [? ?]
+    | H : ~ access _ (TM_Seq _ _) _ |- _ =>
+        eapply inversion_not_access_seq in H as [? ?]
   end.
 
-Lemma access_load_not : forall m t ad,
+Lemma not_access_new : forall m t ad,
+  ~ access m t ad ->
+  ~ access m (TM_New t) ad.
+Proof.
+  intros * ? ?. inversion_access. eauto.
+Qed.
+
+Lemma not_access_load : forall m t ad,
   ~ access m t ad ->
   ~ access m (TM_Load t) ad.
 Proof.
   intros * ? ?. inversion_access. eauto.
 Qed.
 
-Lemma access_asg_not : forall m l r ad,
+Lemma not_access_asg : forall m l r ad,
   ~ access m l ad /\ ~ access m r ad ->
   ~ access m (TM_Asg l r) ad.
 Proof.
   intros * [? ?] ?. inversion_access; eauto.
 Qed.
 
-Lemma access_seq_not : forall m t1 t2 ad,
+Lemma not_access_seq : forall m t1 t2 ad,
   ~ access m t1 ad /\ ~ access m t2 ad ->
   ~ access m (TM_Seq t1 t2) ad.
 Proof.
   intros * [? ?] ?. inversion_access; eauto.
 Qed.
 
+(* Properties of access over step. *)
+
+Local Lemma memory_add_preserves_access : forall m t ad v,
+  access m t ad ->
+  access (add m v) t ad.
+Proof.
+  intros * Hacc. induction Hacc; eauto using access.
+  eapply access_mem. destruct (lt_eq_lt_dec ad' (length m)) as [[? | ?] | ?]. 
+  - rewrite (get_add_lt TM_Nil); trivial.
+  - subst. rewrite (get_default TM_Nil) in IHHacc; eauto using Nat.le_refl.
+    inversion_access.
+  - rewrite (get_default TM_Nil) in IHHacc; eauto using Nat.lt_le_incl.
+    inversion_access.
+Qed.
+
+Local Lemma memory_set_preserves_access : forall m t ad ad' v,
+  ~ access m v ad ->
+  access (set m ad' v) t ad ->
+  access m t ad.
+Proof.
+  intros * Hnacc Hacc. remember (set m ad' v) as m'.
+  induction Hacc; inversion Heqm'; subst; eauto using access.
+  match goal with 
+    IH : ~ _ -> access _ (getTM (set _ ?ad1 _) ?ad2) ?ad3 |- _ =>
+      destruct (Nat.eq_dec ad1 ad2); subst;
+      try solve [rewrite (get_set_neq TM_Nil) in IH; eauto using access];
+      destruct (Nat.eq_dec ad2 ad3); subst; eauto using access
+  end.
+  exfalso. rewrite (get_set_eq TM_Nil) in IHHacc; eauto.
+  eapply not_le. intros F. rewrite (get_default TM_Nil) in Hacc.
+  - inversion_access.
+  - rewrite set_preserves_length. trivial.
+Qed.
+
+Ltac induction_step :=
+  match goal with
+    | H : _ --[_]--> _ |- _ => induction H
+  end.
+
+Lemma mstep_none_does_not_grant_access : forall m m' t t' ad,
+  access m' t' ad ->
+  m / t ==[EF_None]==> m' / t' ->
+  access m t ad.
+Proof.
+  intros * Hacc Hmstep. inversion Hmstep; subst; clear Hmstep.
+  remember EF_None as eff. induction_step; inversion Heqeff; subst;
+  try inversion_access; eauto using access.
+Qed.
+
+Lemma mstep_load_does_not_grant_access : forall m m' t t' ad ad' v,
+  access m' t' ad ->
+  m / t ==[EF_Load ad' v]==> m' / t' ->
+  access m t ad.
+Proof.
+  intros * Hacc Hmstep. inversion Hmstep; subst; clear Hmstep.
+  remember (EF_Load ad' (getTM m' ad')) as eff. 
+  induction_step; inversion Heqeff; subst;
+  try inversion_access; eauto using access.
+Qed.
+
+Lemma mstep_store_does_not_grant_access : forall m m' t t' ad ad' v,
+  access m' t' ad ->
+  m / t ==[EF_Store ad' v]==> m' / t' ->
+  access m t ad.
+Proof.
+  intros * Hacc Hmstep. inversion Hmstep; subst; clear Hmstep.
+  remember (EF_Store ad' v) as eff. 
+  induction_step; inversion Heqeff; subst;
+  try inversion_access; eauto using access.
+  - eapply access_asg2.
+Qed.
+
+
+
+
+
+
+
+
+
+
+
+
+
+
+
+
+Lemma alloc_preserves_access : forall m m' t t' ad ad' v,
+  access m t ad ->
+  m / t ==[EF_Alloc ad' v]==> m' / t' ->
+  access m' t' ad.
+Proof.
+  intros * Hacc Hmstep. inversion Hmstep; subst; clear Hmstep.
+  remember (EF_Alloc (length m) v) as eff.
+  induction_step; inversion Heqeff; subst; inversion_access;
+  eauto using access, memory_add_preserves_access.
+  eapply access_mem. rewrite (get_add_eq TM_Nil).
+  eauto using memory_add_preserves_access.
+Qed.
+
+Lemma when_load_preserves_access : forall m m' t t' ad ad' v,
+  ad <> ad' ->
+  access m t ad ->
+  m / t ==[EF_Load ad' v]==> m' / t' ->
+  access m' t' ad.
+Proof.
+  intros * Hneq Hacc Hmstep. inversion Hmstep; subst; clear Hmstep.
+  remember (EF_Load ad' (getTM m' ad')) as eff.
+  induction_step; inversion Heqeff; subst; inversion_access; eauto using access.
+  inversion_access; subst; trivial. exfalso. eauto.
+Qed.
+
+Lemma when_store_preserves_access : forall m m' t t' ad ad' v,
+  ad <> ad' ->
+  access m t ad ->
+  m / t ==[EF_Store ad' v]==> m' / t' ->
+  access m' t' ad.
+Proof.
+  intros * Hneq Hacc Hmstep. inversion Hmstep; subst; clear Hmstep.
+  remember (EF_Store ad' v) as eff.
+  induction_step; inversion Heqeff; subst; inversion_access;
+  eauto using access.
+  - eapply access_asg2.
+Abort.
 
 (*
-Ltac destruct_access_H H :=
-  idtac H;
-  match type of H with
-    | access _ TM_Nil _ => inversion H
-    | access _ (TM_Num _) _ => inversion H
-    | access _ (TM_New _) _ => eapply new_access in H
-  end.
+  | EF_Alloc (ad : addr) (t : tm)
+  | EF_Load  (ad : addr) (t : tm)
+  | EF_Store (ad : addr) (t : tm)
 *)
